src/Language/PlutusIR/Semantics/SemanticEquivalence/CompatibilityLemmas/LetNonRec.v
@@ -50,24 +50,16 @@ Proof.
       assumption.
 Qed.
 
-(*
-Lemma subst_bs_nr__bound_vars : forall x s bs bs',
-    substitute_bindings_nonrec x s bs bs' ->
-    term_vars_bound_by_bindings bs = term_vars_bound_by_bindings bs'.
-Proof.
-  intros.
-  induction H.
-  - reflexivity.
-  - destruct b. 
-    all: inversion H0; subst.
-    all: auto.
-  - destruct b.
-    all: inversion H0. subst.
-    all: unfold term_vars_bound_by_bindings.
-    all: simpl.
-    all: f_equal.
-    all: auto.
-Qed.*)
+Lemma substb__bound_vars : forall x s b b',
+    substitute_binding x s b b' ->
+    bound_vars_in_binding b = bound_vars_in_binding b'.
+Proof. intros. induction H. all: eauto. Qed.
+
+
+Lemma substAb__bound_tyvars : forall x s b b',
+    substituteA_binding x s b b' ->
+    bound_tyvars_in_binding b = bound_tyvars_in_binding b'.
+Proof. intros. induction H. all: eauto. Qed.
 
 Lemma substA_bs_nr__bound_tyvars : forall x s bs bs',
     substituteA_bindings_nonrec x s bs bs' ->
@@ -87,180 +79,564 @@ Proof.
     apply IHsubstituteA_bindings_nonrec.
 Qed.
     
-(*
-Lemma msubst_LetNonRec : forall ss bs e t',
-    msubst_term ss (Let NonRec bs e) t' ->
-    exists bs' e', 
-      ForallP (fun b => exists b, msubst )
-      msubst_bindings_nonrec ss bs bs' /\ 
-      msubst_term (mdrop (term_vars_bound_by_bindings bs) ss) e e' /\ 
-      t' = Let NonRec bs' e'.
+Lemma msubst_LetNonRec_nil : forall ss e t',
+    msubst_term ss (Let NonRec nil e) t' ->
+    exists e',
+      msubst_term ss e e' /\
+      t' = Let NonRec nil e'.
 Proof.
   induction ss; intros.
   - inversion H. subst.
-    exists bs, e.
-    rewrite mdrop_nil.
-    eauto using msubst_bindings_nonrec__nil, msubst_nil, msubst_cons. 
+    exists e.
+    eauto using msubst_term__nil.
   - inversion H. subst.
+    rename t'0 into t''.
+    inversion H2. subst.
     rename t'0 into e''.
+    apply IHss in H5.
+    destruct H5 as [e' [Hms__e' Heq]].
+    subst.
+    eauto using msubst_term__cons.
+Qed.
+
+Lemma msubst_LetNonRec_cons : forall ss b bs e t',
+    msubst_term ss (Let NonRec (b :: bs) e) t' ->
+    exists b' bs' e',
+      msubst_binding ss b b' /\
+      msubst_term (mdrop (bound_vars_in_binding b) ss) (Let NonRec bs e) (Let NonRec bs' e') /\
+      t' = Let NonRec (b' :: bs') e'.
+Proof.
+  induction ss; intros.
+  - inversion H. subst.
+    exists b, bs, e.
+    rewrite mdrop_nil.
+    eauto using msubst_term__nil, msubst_binding__nil.
+  - inversion H. subst.
+    rename t'0 into t''.
     inversion H2.
     + subst.
-      apply IHss in H5.
-      destruct H5 as [bs'' [e'' [H9 [H10 H11]]]].
+      eapply IHss in H5 as H8.
+      destruct H8 as [b'' [bs'' [e'' [Hms__b'' [Hms__t'' Heq]]]]].
       subst.
-      exists bs'', e''.
+      exists b''.
+      exists bs''.
+      exists e''.
       split. {
-        apply msubst_bindings_nonrec__cons with bs'.
-        + assumption.
-        + apply H9.
+        eapply msubst_binding__cons.
+        all: eassumption.
       }
       split. {
-        rewrite In__mdrop; auto.
-        erewrite subst_bs_nr__bound_vars; eauto.
+        rewrite In__mdrop.
+        - erewrite substb__bound_vars.
+          all: eassumption.
+        - eassumption.
       }
       reflexivity.
     + subst.
-      rename t0' into e'.
-      apply IHss in H5.
-      destruct H5 as [bs'' [e'' [H10 [H11 H12]]]].
+      eapply IHss in H5 as H9.
+      destruct H9 as [b'' [bs'' [e'' [Hms__b'' [Hms__t'' Heq]]]]].
       subst.
-      exists bs'', e''.
+      exists b''.
+      exists bs''.
+      exists e''.
       split. {
-        apply msubst_bindings_nonrec__cons with bs'.
-        + assumption.
-        + apply H10.
+        eapply msubst_binding__cons.
+        all: eassumption.
       }
       split. {
-        rewrite not_In__mdrop; auto.
-        eapply msubst_cons; eauto. 
-        erewrite subst_bs_nr__bound_vars; eauto.
+        rewrite not_In__mdrop.
+        - erewrite substb__bound_vars.
+          + eapply msubst_term__cons.
+            all: eassumption.
+          + eassumption.
+        - eassumption.
       }
       reflexivity.
 Qed.
 
-Lemma msubstA_LetNonRec : forall ss bs e t',
-    msubstA ss (Let NonRec bs e) t' ->
-    exists bs' e', 
-      msubstA_bindings_nonrec ss bs bs' /\ 
-      msubstA (mdrop (tyvars_bound_by_bindings bs) ss) e e' /\ 
-      t' = Let NonRec bs' e'.
+Lemma msubst_TermBind : forall ss stricty x T e b',
+    msubst_binding ss (TermBind stricty (VarDecl x T) e) b' ->
+    exists e',
+      msubst_term ss e e' /\
+      b' = TermBind stricty (VarDecl x T) e'.
 Proof.
   induction ss; intros.
   - inversion H. subst.
-    exists bs, e.
-    rewrite mdrop_nil.
-    eauto using msubstA_bindings_nonrec__nil, msubstA_nil, msubstA_cons. 
+    eauto using msubst_term__nil.
   - inversion H. subst.
-    rename t'0 into e''.
+    inversion H2. subst.
+    eapply IHss in H5.
+    destruct H5 as [e'' [Hms__e'' Heq]].
+    eauto using msubst_term__cons.
+Qed.
+
+Lemma msubstA_LetNonRec_nil : forall ss e t',
+    msubstA ss (Let NonRec nil e) t' ->
+    exists e',
+      msubstA ss e e' /\
+      t' = Let NonRec nil e'.
+Proof.
+  induction ss; intros.
+  - inversion H. subst.
+    exists e.
+    eauto using msubstA_nil.
+  - inversion H. subst.
+    rename t'0 into t''.
     inversion H2.
     + subst.
-      apply IHss in H5.
-      destruct H5 as [bs'' [e'' [H9 [H10 H11]]]].
-      subst.
-      exists bs'', e''.
-      split. {
-        apply msubstA_bindings_nonrec__cons with bs'.
-        + assumption.
-        + apply H9.
-      }
-      split. {
-        rewrite In__mdrop; auto.
-        erewrite substA_bs_nr__bound_tyvars; eauto.
-      }
-      reflexivity.
+      destruct H6.
     + subst.
-      rename t0' into e'.
+      inversion H7. subst.
+      rename t0' into e''.
       apply IHss in H5.
-      destruct H5 as [bs'' [e'' [H10 [H11 H12]]]].
+      destruct H5 as [e' [Hmsa__e' Heq]].
       subst.
-      exists bs'', e''.
-      split. {
-        apply msubstA_bindings_nonrec__cons with bs'.
-        + assumption.
-        + apply H10.
-      }
-      split. {
-        rewrite not_In__mdrop; auto.
-        eapply msubstA_cons; eauto. 
-        erewrite substA_bs_nr__bound_tyvars; eauto.
-      }
-      reflexivity.
-Qed. *)
+      eauto using msubstA_cons.
+Qed.
 
-Lemma compatibility_LetNonRec : forall Delta Gamma bs t bs' t' T,
+Lemma msubstA_LetNonRec_cons : forall ss b bs e t',
+    msubstA ss (Let NonRec (b :: bs) e) t' ->
+    exists b' bs' e',
+      msubstA_binding ss b b' /\
+      msubstA (mdrop (bound_tyvars_in_binding b) ss) (Let NonRec bs e) (Let NonRec bs' e') /\
+      t' = Let NonRec (b' :: bs') e'.
+Proof.
+  induction ss; intros.
+  - inversion H. subst.
+    exists b, bs, e.
+    rewrite mdrop_nil.
+    eauto using msubstA_nil, msubstA_binding__nil.
+  - inversion H. subst.
+    rename t'0 into t''.
+    inversion H2.
+    + subst.
+      inversion H8.
+      * subst.
+        eapply IHss in H5 as H9.
+        destruct H9 as [b'' [bs'' [e'' [Hmsa__b'' [Hmsa__t'' Heq]]]]].
+        subst.
+        exists b''.
+        exists bs''.
+        exists e''.
+        split. {
+          eapply msubstA_binding__cons.
+          all: eassumption.
+        }
+        split. {
+          rewrite In__mdrop.
+          - erewrite substAb__bound_tyvars.
+            all: eassumption.
+          - eassumption.
+        }
+        reflexivity.
+      * subst.
+        unfold bound_tyvars_in_bindings in H6.
+        simpl in H6.
+        apply List.in_app_or in H6.
+        destruct H6.
+        -- exfalso. auto.
+        -- eapply IHss in H5 as H12.
+           destruct H12 as [b'' [bs'' [e'' [Hmsa__b'' [Hmsa__t'' Heq]]]]].
+           subst.
+           exists b''.
+           exists bs''.
+           exists e''.
+           split. {
+             eapply msubstA_binding__cons.
+             all: eassumption.
+           }
+           split. {
+             rewrite not_In__mdrop.
+             - eapply msubstA_cons.
+               + eapply SA_Let1; eauto.
+               + erewrite substAb__bound_tyvars.
+                all: eassumption.
+             - eassumption.
+           }
+          reflexivity.
+    + subst.
+      inversion H7.
+      * subst.
+        exfalso.
+        apply H3.
+        unfold bound_tyvars_in_bindings.
+        simpl.
+        apply List.in_or_app.
+        left.
+        assumption.
+      * subst.
+        eapply IHss in H5 as H13.
+        destruct H13 as [b'' [bs'' [e'' [Hms__b'' [Hms__t'' Heq]]]]].
+        subst.
+        exists b''.
+        exists bs''.
+        exists e''.
+        split. {
+          eapply msubstA_binding__cons.
+          all: eassumption.
+        }
+        split. {
+          rewrite not_In__mdrop.
+          - eapply msubstA_cons.
+            + eapply SA_Let2; eauto.
+              intros Hcon.
+              apply H3.
+              unfold bound_tyvars_in_bindings.
+              simpl.
+              apply List.in_or_app.
+              right.
+              assumption.
+            + erewrite substAb__bound_tyvars.
+            all: eassumption.
+          - eassumption.
+        }
+        reflexivity.
+Qed.
+
+Lemma msubstA_TermBind : forall ss stricty x T e b',
+    msubstA_binding ss (TermBind stricty (VarDecl x T) e) b' ->
+    exists e',
+      msubstA ss e e' /\
+      b' = TermBind stricty (VarDecl x (msubstT ss T)) e'.
+Proof.
+  induction ss; intros.
+  - inversion H. subst.
+    eauto using msubstA_nil.
+  - inversion H. subst.
+    inversion H2. subst.
+    eapply IHss in H5.
+    destruct H5 as [e'' [Hmsa__e'' Heq]].
+    eauto using msubstA_cons.
+Qed.
+
+Lemma inspect_eval__LetNonRec_nil : forall e j e_f,
+    Let NonRec nil e =[j]=> e_f ->
+    exists j_1, e =[j_1]=> e_f /\ j = j_1 + 1.
+Proof.
+  intros.
+  inversion H. subst.
+  inversion H4. subst.
+  exists k.
+  split.
+  - assumption.
+  - rewrite plus_comm.
+    reflexivity.
+Qed.
+
+Lemma inspect_eval__LetNonRec_cons : forall s x T eb bs e j e_f,
+    Let NonRec (TermBind s (VarDecl x T) eb :: bs) e =[j]=> e_f ->
+    exists j_1 eb_f, 
+      eb =[j_1]=> eb_f /\ j_1 <= j /\
+      exists bs' e',
+        substitute x eb_f (Let NonRec bs e) (Let NonRec bs' e') /\
+        exists j_2,
+          Let NonRec bs' e' =[j_2]=> e_f /\
+          j_1 + 1 + j_2 = j.
+Proof.
+  intros.
+  inversion H. subst.
+  inversion H4. subst.
+  exists kb, vb.
+  split. auto.
+  split. apply skip. (* TODO*)
+  exists bs', t'.
+  split. auto.
+  exists k.
+  split. apply E_Let. auto.
+  reflexivity.
+Qed.
+
+Lemma compatibility_LetNonRec : forall bs Delta Gamma t bs' t' T,
     forall Delta' Gamma',
       (Delta', Gamma') = append (flatten (List.map binds bs)) (Delta, Gamma) ->
       LR_logically_approximate Delta' Gamma' t t' T ->
       LR_logically_approximate_bindings_nonrec Delta Gamma bs bs' ->
       LR_logically_approximate Delta Gamma (Let NonRec bs t) (Let NonRec bs' t') T.
 Proof.
-  intros Delta Gamma bs t bs' t' T Delta' Gamma' Hbinds IH_LR__t IH_LR__bs.
-  unfold LR_logically_approximate.
+  induction bs.
+  - intros Delta Gamma t bs' t' T Delta' Gamma' Hbinds IH_LR__t IH_LR__bs.
+    unfold LR_logically_approximate.
 
-  split. {
-    eapply T_Let. 
-    - apply Hbinds.
-    - eapply LR_la_bnr__oks in IH_LR__bs. 
-      apply IH_LR__bs. 
-    - apply IH_LR__t.  
-  }
+    inversion IH_LR__bs. subst.
 
-  split. {
-    eapply T_Let.
-    - eapply LR_la_bnr__oks in IH_LR__bs.
-      destruct IH_LR__bs as [_ [_ Heq]].
-      rewrite <- Heq.
-      apply Hbinds.
-    - eapply LR_la_bnr__oks in IH_LR__bs.
-      apply IH_LR__bs.
-    - apply IH_LR__t.
-  }
+    split. {
+      eapply T_Let.
+      all: eauto with typing.
+      unfold LR_logically_approximate in IH_LR__t.
+      apply IH_LR__t.
+    }
 
-  intros k rho env env' ct ck HeqDelta HeqGamma [H_RD H_RG].
-  subst.
+    split. {
+      eapply T_Let.
+      all: eauto with typing.
+      unfold LR_logically_approximate in IH_LR__t.
+      apply IH_LR__t.
+    }
 
-  intros e_msa e'_msa e_ms e'_ms.
-  intros HmsA__e_msa HmsA__e'_msa Hms__e_ms Hms__e'_ms.
+    intros k rho env env' ct ck HeqDelta HeqGamma [H_RD H_RG].
+    subst.
 
-  (*
-  destruct (msubstA_LetNonRec _ _ _ _ HmsA__e_msa) as [bs_msa [t_msa [HmsA__bs_msa [HmsA__t_msa Heq]]]].
-  destruct (msubstA_LetNonRec _ _ _ _ HmsA__e'_msa) as [bs'_msa [t'_msa [HmsA__bs'_msa [HmsA__t'_msa Heq']]]].
-  subst.
-  destruct (msubst_LetNonRec _ _ _ _ Hms__e_ms) as [bs_ms [t_ms [Hms__bs_ms [Hms__t_ms Heq]]]].
-  destruct (msubst_LetNonRec _ _ _ _ Hms__e'_ms) as [bs'_ms [t'_ms [Hms__bs'_ms [Hms__t'_ms Heq']]]].
-  subst.
+    intros e_msa e'_msa e_ms e'_ms.
+    intros Hmsa__e_msa Hmsa__e'_msa Hms__e_ms Hms__e'_ms.
 
-  autorewrite with RC.
-  split. {
-    replace emptyContext with (@empty Kind, mupd (msyn1 rho) empty).
-    - eapply msubst_preserves_typing_1; eauto.
-      eapply msubstA_preserves_typing_1; eauto.
-      eapply T_Let; eauto.
-      + eapply LR_la_bnr__oks in IH_LR__bs. 
-        apply IH_LR__bs.
-      + eapply IH_LR__t.
-    - rewrite mupd_empty; eauto.
-  }
-  split. {
-    replace emptyContext with (@empty Kind, mupd (msyn2 rho) empty).
-    - eapply LR_la_bnr__oks in IH_LR__bs as H.
-      eapply msubst_preserves_typing_2; eauto.
-      eapply msubstA_preserves_typing_2; eauto.
-      eapply T_Let; eauto.
-      + apply H.
-      + destruct H. destruct H0. 
-        rewrite <- H1.
-        Fail rewrite <- Hbinds. (* why?? *)
-        unfold LR_logically_approximate in IH_LR__t.
-        apply skip.
-    - rewrite mupd_empty; eauto.
-  }
+    destruct (msubstA_LetNonRec_nil _ _ _ Hmsa__e_msa) as [t_msa [Hmsa__t_msa Heq]].
+    destruct (msubstA_LetNonRec_nil _ _ _ Hmsa__e'_msa) as [t'_msa [Hmsa__t'_msa Heq']].
+    subst.
+    destruct (msubst_LetNonRec_nil _ _ _ Hms__e_ms) as [t_ms [Hms__t_ms Heq]].
+    destruct (msubst_LetNonRec_nil _ _ _ Hms__e'_ms) as [t'_ms [Hms__t'_ms Heq']].
+    subst.
 
-  intros j Hlt__j e_f Hev__e_f.
-  inversion Hev__e_f. subst.
-  inversion H3. subst.
-  - unfold LR_logically_approximate in IH_LR__t.
+    autorewrite with RC.
+
+    split. {
+      replace emptyContext with (@empty Kind, mupd (msyn1 rho) empty).
+      - eapply msubst_preserves_typing_1; eauto.
+        eapply msubstA_preserves_typing_1; eauto.
+        eapply T_Let; eauto with typing. 
+        eapply IH_LR__t.
+      - rewrite mupd_empty; eauto.
+    }
+    split. {
+      replace emptyContext with (@empty Kind, mupd (msyn2 rho) empty).
+      - eapply msubst_preserves_typing_2; eauto.
+        eapply msubstA_preserves_typing_2; eauto.
+        eapply T_Let; eauto with typing. 
+        eapply IH_LR__t.
+      - rewrite mupd_empty; eauto.
+    }
+
+    intros j Hlt__j e_f Hev__e_f.
+    apply inspect_eval__LetNonRec_nil in Hev__e_f as temp.
+    destruct temp as [j_1 [Hev'__e_f Heq]].
+    
     destruct IH_LR__t as [_ [_ IH_LR__t]].
-    inversion Hbinds. subst. 
-  *)
+    assert (RC k T rho t_ms t'_ms). {
+      simpl in Hbinds.
+      rewrite flatten_nil in Hbinds.
+      rewrite append_emptyContext_l in Hbinds.
+      inversion Hbinds. subst.
+      eapply IH_LR__t.
+      all: eauto.
+    }
+
+    autorewrite with RC in H.
+    destruct H as [_ [_ H]].
+
+    assert (Hlt__j_1 : j_1 < k). {
+      subst. 
+      rewrite plus_comm in Hlt__j.
+      apply Nat.succ_lt_mono.
+      apply le_S.
+      assumption.
+    }
+    remember (H j_1 Hlt__j_1 e_f Hev'__e_f).
+    clear Heqe. rename e into H0.
+
+    destruct H0 as [e'_f [j'_1 [Hev__e'_f H0]]].
+    exists e'_f. exists (S j'_1).
+    split. {
+      eapply E_Let.
+      eapply E_NilB_NonRec.
+      eassumption.
+    }
+
+    assert (forall i, i < k - j -> i < k - j_1). { 
+      intros.
+      subst.
+      rewrite plus_comm in H1.
+      simpl in H1.
+      apply skip. 
+    }
+
+    destruct T.
+    all: eauto.
+    intros.
+    eapply RD_sem_syn in H2 as H3; eauto.
+    destruct H3 as [T1 [T2 [Hsyn1 Hsyn2]]].
+    apply H0 in H2 as H3; eauto.
+    eapply RD_rel in H2; eauto.
+    unfold Rel in H2.
+    eapply H2; eauto.
+    subst.
+    apply skip.
+
+  - intros Delta Gamma t bs' t' T Delta' Gamma' Hbinds IH_LR__t IH_LR__bbs.
+    unfold LR_logically_approximate.
+    rename a into b.
+    remember IH_LR__t as IH_LR__t__copy.
+    clear HeqIH_LR__t__copy.
+
+    inversion IH_LR__bbs. subst.
+    rename bs'0 into bs'.
+    rename Delta'0 into Delta''.
+    rename Gamma'0 into Gamma''.
+    rename H1 into IH_LR__b.
+    rename H2 into Hbinds''.
+    rename H5 into Heqbinds.
+    rename H7 into IH_LR__bs.
+
+    assert (IH_LR__let : LR_logically_approximate Delta'' Gamma'' (Let NonRec bs t) (Let NonRec bs' t') T). {
+      eapply IHbs.
+      all: eauto.
+      apply skip. (* TODO *)
+    }
+    remember IH_LR__let as IH_LR__let__copy.
+    clear HeqIH_LR__let__copy.
+
+    split. {
+      eapply T_Let. 
+      - apply Hbinds.
+      - eapply LR_la_bnr__oks in IH_LR__bbs. 
+        apply IH_LR__bbs. 
+      - apply IH_LR__t.  
+    }
+
+    split. {
+      eapply T_Let.
+      - eapply LR_la_bnr__oks in IH_LR__bbs.
+        destruct IH_LR__bbs as [_ [_ Heq]].
+        rewrite <- Heq.
+        apply Hbinds.
+      - eapply LR_la_bnr__oks in IH_LR__bbs.
+        apply IH_LR__bbs.
+      - apply IH_LR__t.
+    }
+
+    intros k rho env env' ct ck HeqDelta HeqGamma [H_RD H_RG].
+    subst.
+
+    intros e_msa e'_msa e_ms e'_ms.
+    intros Hmsa__e_msa Hmsa__e'_msa Hms__e_ms Hms__e'_ms.
+
+    destruct (msubstA_LetNonRec_cons _ _ _ _ _ Hmsa__e_msa) as [b_msa [bs_msa [t_msa [Hmsa__b_msa [Hmsa__eih_msa Heq]]]]].
+    destruct (msubstA_LetNonRec_cons _ _ _ _ _ Hmsa__e'_msa) as [b'_msa [bs'_msa [t'_msa [Hmsa__b'_msa [Hmsa__eih'_msa Heq']]]]].
+    subst.
+
+    destruct (msubst_LetNonRec_cons _ _ _ _ _ Hms__e_ms) as [b_ms [bs_ms [t_ms [Hms__b_ms [Hms__eih_ms Heq]]]]].
+    destruct (msubst_LetNonRec_cons _ _ _ _ _ Hms__e'_ms) as [b'_ms [bs'_ms [t'_ms [Hms__b'_ms [Hms__eih'_ms Heq']]]]].
+    subst.
+
+    autorewrite with RC.
+    split. {
+      replace emptyContext with (@empty Kind, mupd (msyn1 rho) empty).
+      - eapply msubst_preserves_typing_1; eauto.
+        eapply msubstA_preserves_typing_1; eauto.
+        eapply T_Let; eauto.
+        + eapply LR_la_bnr__oks in IH_LR__bbs. 
+          apply IH_LR__bbs.
+        + eapply IH_LR__t.
+      - rewrite mupd_empty; eauto.
+    }
+    split. {
+      replace emptyContext with (@empty Kind, mupd (msyn2 rho) empty).
+      - eapply LR_la_bnr__oks in IH_LR__bbs as H.
+        eapply msubst_preserves_typing_2; eauto.
+        eapply msubstA_preserves_typing_2; eauto.
+        eapply T_Let; eauto.
+        + apply H.
+        + destruct H. destruct H0. 
+          rewrite <- H1.
+          unfold LR_logically_approximate in IH_LR__t.
+          inversion Hbinds. subst.
+          apply IH_LR__t.
+      - rewrite mupd_empty; eauto.
+    }
+
+    assert (H_RB : RB k rho b_ms b'_ms) by (eapply IH_LR__b; eauto).
+    autorewrite with RB in H_RB.
+
+    destruct b, b'.
+    + destruct v.
+      rename s into stricty.
+      rename s1 into x.
+      rename t2 into Tb.
+      rename t0 into eb.
+    
+      destruct v0.
+      rename s0 into stricty'.
+      rename s into x'.
+      rename t0 into Tb'.
+      rename t1 into eb'.
+      
+      assert (x' = x /\ Tb' = Tb). {
+        inversion Heqbinds.
+        apply skip.
+      }
+
+      destruct H.
+      subst.
+
+      destruct (msubstA_TermBind _ _ _ _ _ _ Hmsa__b_msa) as [eb_msa [Hmsa__eb_msa Heq]].
+      destruct (msubstA_TermBind _ _ _ _ _ _ Hmsa__b'_msa) as [eb'_msa [Hmsa__eb'_msa Heq']].
+      subst.
+      destruct (msubst_TermBind _ _ _ _ _ _ Hms__b_ms) as [eb_ms [Hms__eb_ms Heq]].
+      destruct (msubst_TermBind _ _ _ _ _ _ Hms__b'_ms) as [eb'_ms [Hms__eb'_ms Heq']].
+      subst.
+
+      intros j Hlt__j e_f Hev__e_f.
+      apply inspect_eval__LetNonRec_cons in Hev__e_f as temp.
+      destruct temp as [j_1 [eb_f [Hev__eb_f [Hle__j_1 [bs0 [t0 [Hsubs__ih [j_2 [Hev__ih Heq]]]]]]]]].
+      
+      
+      destruct H_RB as [_ [ _ H_RC]].
+      autorewrite with RC in H_RC.
+
+      destruct H_RC as [_ [_ H_RC]].
+      assert (Hlt__j_1 : j_1 < k). { apply skip. }
+      remember (H_RC j_1 Hlt__j_1 eb_f Hev__eb_f).
+      clear Heqe. clear H_RC. rename e into H_RC.
+
+      destruct H_RC as [eb'_f [j'_1 [Hev__eb'_f H_RC]]].
+      clear H_RC.
+
+      simpl in Hms__eih_ms.
+      assert (msubst_term ((x, eb_f) :: env) (Let NonRec bs_msa t_msa) (Let NonRec bs0 t0)). {
+        apply skip.
+      }
+      simpl in Hms__eih'_ms.
+      assert (exists bs0' t0', substitute x eb'_f (Let NonRec bs'_ms t'_ms) (Let NonRec bs0' t0')). {
+        apply skip.
+      }
+      destruct H0 as [bs0' [t0' H1]].
+      assert (msubst_term ((x, eb'_f) :: env') (Let NonRec bs'_msa t'_msa) (Let NonRec bs0' t0')). {
+        apply skip.
+      }
+       
+      destruct IH_LR__let as [_ [_ IH_LR__let]].
+      assert (RC k T rho (Let NonRec bs0 t0) (Let NonRec bs0' t0')). {
+        eapply IH_LR__let.
+        - apply skip.
+        - apply skip.
+        - split. eassumption.
+          eapply RG_cons. 
+          all: apply skip.
+        - eassumption.
+        - eassumption.
+        - eassumption.
+        - eassumption.
+      }
+
+      autorewrite with RC in H2.
+      destruct H2 as [_ [_ H2]].
+      assert (Hlt__j_2 : j_2 < k). {  apply skip. }
+      remember (H2 _ Hlt__j_2 _ Hev__ih).
+      clear Heqe. clear H2. rename e into H2.
+      destruct H2 as [e'_f [j'_2 [Hev__e'_f H2]]].
+
+      eexists. eexists.
+      split. {
+        eapply E_Let.
+        eapply E_ConsB_NonRec.
+        all: eauto.
+        inversion Hev__e'_f.
+        subst.
+        eauto.
+      }
+
+      assert (forall i, i < k - j -> i < k - j_2). { apply skip. } 
+
+      destruct T.
+      all: eauto.
+      apply skip.
+    +
 Admitted.
