src/Language/PlutusIR/Semantics/SemanticEquivalence/FundamentalProperty.v
@@ -2,11 +2,8 @@ Require Import PlutusCert.Language.PlutusIR.
 Import NamedTerm.
 Require Import PlutusCert.Language.PlutusIR.Semantics.Dynamic.
 Require Import PlutusCert.Language.PlutusIR.Semantics.Static.
-Require Import PlutusCert.Language.PlutusIR.Semantics.TypeSafety.Preservation.
-Require Import PlutusCert.Language.PlutusIR.Semantics.TypeSafety.SubstitutionPreservesTyping.
 Require Import PlutusCert.Language.PlutusIR.Semantics.SemanticEquivalence.CompatibilityLemmas.
 Require Import PlutusCert.Language.PlutusIR.Semantics.SemanticEquivalence.LogicalRelation.RelationalModel.
-Require Import PlutusCert.Language.PlutusIR.Semantics.SemanticEquivalence.Monotonicity.
 Require Import PlutusCert.Util.
 
 (** ** The [R] Lemma *)
